oPCF/Utility.lean
@@ -2,10 +2,6 @@ def Nat.zero? : Nat → Bool
 | .zero => true
 | _ => false
 
-theorem Nat.pred_succ_id : Nat.pred ∘ Nat.succ = id := by
-  apply funext
-  exact Nat.pred_succ
-
 infix:100 " ⬝ " => Trans.trans
 
 theorem congrArg2
